fv/acir_lean/AcirLean.lean
@@ -1,6 +1,4 @@
-import AcirLean.Basic
-import AcirLean.Division
-import AcirLean.Overflow
-import AcirLean.Compare
-import AcirLean.Template
-import AcirLean.Bug7895
+import AcirLean.Spec.Claims
+import AcirLean.Proofs.Main
+import AcirLean.Proofs.Compare
+import AcirLean.Examples.Bug7895
